SEL4GraphRefine now completed.
These final changes complete the SEL4GraphRefine process. Some
cleanup remains to be done, especially in SEL4GlobalsSwap, but the
process is now mature and working, and the testing code
in SEL4GraphRefine can be discarded.

Success depends on seL4 commit 97d6bc96d54f1f0beafb25033b03b57ba54a5113
which is compatible with crefine and will be included in the repo
manifest immediately.

tools/asmrefine/ProveGraphRefine.thy
@@ -42,11 +42,6 @@ lemma disjoint_heap_update_globals_swap_rearranged:
   apply (simp add: global_acc_valid_def hrs_mem_update)
   done
 
-lemma double_heap_update_eq:
-  "heap_update p' (h_val hp'' p') hp = hp
-    \<Longrightarrow> heap_update p v hp = hp'
-    \<Longrightarrow> (heap_update p v (heap_update p' (h_val hp'' p') hp)) = hp'"
-  by simp
 
 lemma h_t_valid_orig_and_ptr_safe:
   "h_t_valid d g p \<Longrightarrow> h_t_valid d g p \<and> ptr_safe p d"
@@ -144,6 +139,92 @@ lemma unat_ucast_if_up:
   apply (simp add: is_up_def source_size_def target_size_def word_size)
   done
 
+lemma Collect_const_mem:
+  "(x \<in> (if P then UNIV else {})) = P"
+  by simp
+
+definition word32_truncate_nat :: "nat => word32 \<Rightarrow> word32"
+where
+  "word32_truncate_nat n x = (if unat x \<le> n then x else of_nat n)"
+
+lemma word32_truncate_noop:
+  "unat x < Suc n \<Longrightarrow> word32_truncate_nat n x = x"
+  by (simp add: word32_truncate_nat_def)
+
+lemma fold_of_nat_eq_Ifs_proof:
+  "\<lbrakk> unat (x :: word32) \<notin> set ns \<Longrightarrow> y = z;
+      \<And>n. n \<in> set ns \<Longrightarrow> x = of_nat n \<Longrightarrow> f n = z \<rbrakk>
+    \<Longrightarrow> foldr (\<lambda>n v. if x = of_nat n then f n else v) ns y = z"
+  apply (induct ns)
+   apply simp
+  apply (atomize(full))
+  apply clarsimp
+  done
+
+lemma fold_of_nat_eq_Ifs:
+  "m < 2 ^ 32
+    \<Longrightarrow> foldr (\<lambda>n v. if x = of_nat n then f n else v) [0 ..< m] (f m)
+        = f (unat (word32_truncate_nat m x))"
+  apply (rule fold_of_nat_eq_Ifs_proof)
+   apply (simp_all add: word32_truncate_nat_def unat_of_nat)
+  done
+
+lemma of_int_sint_scast:
+  "of_int (sint x) = scast x"
+  by (simp add: scast_def word_of_int)
+
+ML {*
+fun preserve_skel_conv consts arg_conv ct = let
+    val (hd, xs) = strip_comb (term_of ct)
+    val self = preserve_skel_conv consts arg_conv
+  in if is_Const hd andalso member (op =) consts
+        (fst (dest_Const hd))
+    then  if null xs then Conv.all_conv ct
+        else Conv.combination_conv self self ct
+    else arg_conv ct end
+
+fun fold_of_nat_eq_Ifs ctxt tm = let
+    fun recr (Const (@{const_name If}, _)
+            $ (@{term "op = :: word32 => _"} $ _ $ n) $ y $ z)
+        = (SOME n, y) :: recr z
+      | recr t = [(NONE, t)]
+    val (ns, vs) = recr tm |> map_split I
+    val ns = map_filter I ns |> map (HOLogic.dest_number #> snd)
+    val _ = (ns = (0 upto (length ns - 1)))
+        orelse raise TERM ("fold_of_nat_eq_Ifs: ns", [tm])
+    val _ = length vs > 1
+        orelse raise TERM ("fold_of_nat_eq_Ifs: no If", [tm])
+    val n = @{term "n_hopefully_uniq :: nat"}
+    fun get_pat @{term "0 :: nat"} @{term "Suc 0 :: nat"} = n
+      | get_pat (f $ x) (g $ y) = get_pat f g $ get_pat x y
+      | get_pat (a as Abs (s, T, t)) (a' as Abs (_, T', t'))
+          = ((T = T' orelse raise TERM ("fold_array_conditional: get_pat", [a, a']))
+              ; Abs (s, T, get_pat t t'))
+      | get_pat t t' = (t aconv t' orelse raise TERM ("fold_array_conditional: get_pat", [t, t'])
+              ; t)
+    val pat = lambda n (get_pat (nth vs 0) (nth vs 1))
+    val thy = Proof_Context.theory_of ctxt
+    val m = HOLogic.mk_number @{typ nat} (length vs - 1)
+    val conv = preserve_skel_conv [fst (dest_Const @{term "op ==>"}),
+            @{const_name Trueprop}, fst (dest_Const @{term "op =="}),
+            @{const_name If}]
+        (Simplifier.rewrite ctxt)
+    val thm = @{thm fold_of_nat_eq_Ifs}
+      |> cterm_instantiate [(@{cpat "?f :: nat \<Rightarrow> ?'a"}, cterm_of thy pat),
+          (@{cpat "?m :: nat"}, cterm_of thy m)]
+      |> simplify (put_simpset HOL_basic_ss ctxt
+          addsimprocs [Word_Bitwise_Tac.expand_upt_simproc]
+          addsimps @{thms foldr.simps id_apply o_apply})
+      |> mk_meta_eq
+      |> Conv.fconv_rule conv
+  in thm end
+
+val fold_of_nat_eq_Ifs_simproc = Simplifier.simproc_global_i
+  @{theory} "fold_of_nat_eq_Ifs"
+  [@{term "If (x = 0) y z"}] (try o fold_of_nat_eq_Ifs)
+*}
+
+
 ML {*
 fun wrap_tac tac i t = let
     val t' = Goal.restrict i 1 t
@@ -154,6 +235,8 @@ fun wrap_tac tac i t = let
 
 fun eqsubst_wrap_tac ctxt thms = wrap_tac (EqSubst.eqsubst_tac ctxt [0] thms)
 fun eqsubst_asm_wrap_tac ctxt thms = wrap_tac (EqSubst.eqsubst_asm_tac ctxt [0] thms)
+fun eqsubst_either_wrap_tac ctxt thms = (eqsubst_asm_wrap_tac ctxt thms
+    ORELSE' eqsubst_wrap_tac ctxt thms)
 *}
 
 ML {*
@@ -203,21 +286,6 @@ fun enum_simps csenv ctxt = let
 fun safe_goal_tac ctxt =
   REPEAT_ALL_NEW (DETERM o CHANGED o safe_steps_tac ctxt)
 
-fun heap_upd_kind (Const (@{const_name heap_update}, _) $ _ $ _ $ _)
-    = "HeapUpd"
-  | heap_upd_kind (Const (@{const_name hrs_mem}, _) $ v)
-    = let
-    val gs = exists_Const (fn (s, _) => s = @{const_name globals_swap}) v
-    val hu = exists_Const (fn (s, _) => s = @{const_name heap_update}) v
-  in (gs orelse raise TERM ("heap_upd_kind: hrs_mem but no globals_swap", [v]));
-    if hu then "HeapUpdWithSwap" else "GlobalUpd"
-  end
-  | heap_upd_kind t = raise TERM ("heap_upd_kind: unknown", [t])
-
-fun except_tac ctxt msg = SUBGOAL (fn (t, _) => let
-  in warning msg; Syntax.pretty_term ctxt t |> Pretty.writeln;
-    raise TERM (msg, [t]) end)
-
 fun res_from_ctxt tac_name thm_name ctxt thm = let
     val thm_from_ctxt = Proof_Context.get_thm ctxt thm_name
       handle ERROR _ => raise THM (tac_name ^ ": need thm " ^ thm_name, 1, [])
@@ -226,10 +294,10 @@ fun res_from_ctxt tac_name thm_name ctxt thm = let
         1, [thm_from_ctxt, thm])
   end
 
+val except_tac = SimplToGraphProof.except_tac
+
 fun prove_ptr_safe reason ctxt = DETERM o
-    (TRY o REPEAT_ALL_NEW (eqsubst_asm_wrap_tac ctxt
-                @{thms array_ptr_index_coerce}
-            ORELSE' eqsubst_wrap_tac ctxt
+    (TRY o REPEAT_ALL_NEW (eqsubst_either_wrap_tac ctxt
                 @{thms array_ptr_index_coerce}
             )
         THEN_ALL_NEW asm_simp_tac (ctxt addsimps
@@ -247,8 +315,7 @@ fun get_disjoint_h_val_globals_swap ctxt =
 
 fun prove_heap_update_id ctxt = DETERM o let
     val thm = get_disjoint_h_val_globals_swap ctxt
-  in fn i => (resolve_tac @{thms heap_update_id_Array heap_update_id
-                heap_update_id_Array[symmetric] heap_update_id[symmetric]} i
+  in fn i => (resolve_tac @{thms heap_update_id_Array heap_update_id} i
         ORELSE except_tac ctxt "prove_heap_update_id: couldn't init" i)
     THEN (simp_tac ctxt
     THEN_ALL_NEW (* simp_tac will solve goal unless globals swap involved *)
@@ -286,10 +353,12 @@ fun normalise_mem_accs ctxt = DETERM o let
   in
     asm_full_simp_tac (ctxt addsimps init_simps addsimps [h_val])
     THEN_ALL_NEW
-        (TRY o REPEAT_ALL_NEW ((eqsubst_wrap_tac ctxt
+        (TRY o REPEAT_ALL_NEW ((eqsubst_asm_wrap_tac ctxt
+                    @{thms heap_access_Array_element'}
+                ORELSE' eqsubst_wrap_tac ctxt
                     @{thms heap_access_Array_element'}
                 ORELSE' disjoint_h_val_tac)
-            THEN_ALL_NEW asm_simp_tac (ctxt addsimps init_simps)))
+            THEN_ALL_NEW asm_full_simp_tac (ctxt addsimps init_simps)))
     THEN_ALL_NEW
         SUBGOAL (fn (t, i) => case
             Envir.beta_eta_contract (Logic.strip_assums_concl t)
@@ -298,8 +367,12 @@ fun normalise_mem_accs ctxt = DETERM o let
             | @{term Trueprop} $ (Const (@{const_name ptr_safe}, _) $ _ $ _)
               => prove_ptr_safe "normalise_mem_accs" ctxt i
             | _ => all_tac)
-    THEN_ALL_NEW full_simp_tac (ctxt addsimps @{thms h_val_ptr h_val_word32})
+    THEN_ALL_NEW full_simp_tac (ctxt addsimps @{thms h_val_ptr h_val_word32 h_val_word8})
   end
+
+val heap_update_id_nonsense
+    = Thm.trivial @{cpat "Trueprop
+        (heap_update ?p (h_val ?hp' ?p) (hrs_mem ?hrs) = hrs_mem ?hrs)"}
 
 fun prove_mem_equality ctxt = DETERM o let
     val init_simpset = ctxt
@@ -310,33 +383,34 @@ fun prove_mem_equality ctxt = DETERM o let
     val unpack_simpset = ctxt
         addsimps @{thms heap_update_def to_bytes_array
                heap_update_list_append heap_list_update_ptr heap_list_update_word32
+               h_val_word8 heap_list_update_word8
                field_lvalue_offset_eq ptr_add_def
                array_ptr_index_def
                h_val_word32 h_val_ptr
                take_heap_list_min drop_heap_list_general
-               ucast_nat_def[symmetric]
+               ucast_nat_def of_int_sint_scast
         } @ Proof_Context.get_thms ctxt "field_to_bytes_rewrites"
         addsimprocs [Word_Bitwise_Tac.expand_upt_simproc]
       handle ERROR _ => raise THM
         ("prove_mem_equality: run add_field_to_bytes_rewrites on ctxt", 1, [])
 
-    fun double_heap_update_strategy ctxt =
-        resolve_tac @{thms double_heap_update_eq double_heap_update_eq[THEN sym]}
-            THEN' (TRY o SUBGOAL (fn (_, i) => double_heap_update_strategy ctxt i))
-            THEN' prove_heap_update_id ctxt
+    fun heap_update_id_proofs ctxt = 
+        REPEAT_ALL_NEW (eqsubst_wrap_tac ctxt [heap_update_id_nonsense]
+            THEN' prove_heap_update_id ctxt)
 
   in simp_tac init_simpset
-    THEN_ALL_NEW (TRY o REPEAT_ALL_NEW (eqsubst_wrap_tac ctxt
-        @{thms heap_access_Array_element' heap_update_Array_update}))
-    THEN_ALL_NEW TRY o double_heap_update_strategy ctxt
+    THEN_ALL_NEW (TRY o REPEAT_ALL_NEW ((eqsubst_wrap_tac ctxt
+            @{thms heap_access_Array_element' heap_update_Array_update})
+        THEN_ALL_NEW simp_tac init_simpset))
+    THEN_ALL_NEW TRY o heap_update_id_proofs ctxt
     THEN_ALL_NEW SUBGOAL (fn (t, i) => if
         exists_Const (fn (s, T) => s = @{const_name heap_update}
             andalso get_c_type_size ctxt (domain_type (range_type T)) > 256
         ) t
         then except_tac ctxt "prove_mem_equality: unfolding large heap_update" i
         else all_tac)
-    (* need to normalise mem accs before unfolding unpack_simps
-       as some of this process depends on structured pointer constructions *)
+    (* need to normalise_mem_accs first as it operates on typed pointer ops
+       and won't function after we unpack them *)
     THEN_ALL_NEW normalise_mem_accs ctxt
     THEN_ALL_NEW simp_tac unpack_simpset
     THEN_ALL_NEW simp_tac (ctxt addsimps @{thms store_word32s_equality_fold
@@ -345,7 +419,8 @@ fun prove_mem_equality ctxt = DETERM o let
         addsimps @{thms store_word32s_equality_final add_commute})
     THEN_ALL_NEW SUBGOAL (fn (t, i) => if exists_Const
             (fn (s, _) => s = @{const_name store_word32}
-                orelse s = @{const_name heap_update}) t
+                orelse s = @{const_name heap_update}
+                orelse s = @{const_name heap_update_list}) t
         then except_tac ctxt "prove_mem_equality: remaining mem upds" i
         else all_tac)
   end
@@ -365,6 +440,27 @@ fun clean_heap_upd_swap ctxt = DETERM o let
       ORELSE except_tac ctxt "clean_heap_upd_swap: couldn't atac" i)
     THEN prove_ptr_safe "clean_upd_upd_swap" ctxt i
   end
+
+fun clean_htd_upd_swap ctxt = let
+    val thm = @{thm globals_swap_hrs_htd_update[symmetric]}
+    val thm = res_from_ctxt "clean_htd_upd_swap" "global_acc_valid" ctxt thm
+    val thm = res_from_ctxt "clean_htd_upd_swap" "globals_list_valid" ctxt thm
+  in simp_tac (ctxt addsimps [thm])
+    THEN_ALL_NEW (except_tac ctxt "clean_htd_upd_swap: not finished")
+  end
+
+fun heap_upd_kind (Const (@{const_name heap_update}, _) $ _ $ _ $ _)
+    = "HeapUpd"
+  | heap_upd_kind (Const (@{const_name hrs_mem}, _) $ v)
+    = let
+    val gs = exists_Const (fn (s, _) => s = @{const_name globals_swap}) v
+    val hu = exists_Const (fn (s, _) => s = @{const_name heap_update}) v
+    val htd = exists_Const (fn (s, _) => s = @{const_name hrs_htd_update}) v
+  in (gs orelse raise TERM ("heap_upd_kind: hrs_mem but no globals_swap", [v]));
+    if hu then "HeapUpdWithSwap" else if htd then "HTDUpdateWithSwap"
+        else "GlobalUpd"
+  end
+  | heap_upd_kind t = raise TERM ("heap_upd_kind: unknown", [t])
 
 fun decompose_mem_goals trace ctxt = SUBGOAL (fn (t, i) =>
   case Envir.beta_eta_contract (Logic.strip_assums_concl t) of
@@ -387,6 +483,10 @@ fun decompose_mem_goals trace ctxt = SUBGOAL (fn (t, i) =>
             rtac @{thm sym} i THEN clean_heap_upd_swap ctxt i THEN prove_mem_equality ctxt i
         | ("HeapUpd", "GlobalUpd") => prove_global_equality ctxt i
         | ("GlobalUpd", "HeapUpd") => prove_global_equality ctxt i
+        | ("HTDUpdateWithSwap", _)
+            => clean_htd_upd_swap ctxt i
+        | (_, "HTDUpdateWithSwap")
+            => rtac @{thm sym} i THEN clean_htd_upd_swap ctxt i
         | _ => raise TERM ("decompose_mem_goals: mixed up "
             ^ heap_upd_kind x ^ "," ^ heap_upd_kind y, [x, y])
       end
@@ -411,7 +511,7 @@ fun tactic_check' (ss, t) = (ss, tactic_check (hd ss) t)
 
 fun graph_refine_proof_tacs csenv ctxt = let
     (* FIXME: fix shiftr_no and sshiftr_no in Word *)
-    val ctxt = ctxt delsimps @{thms shiftr_no sshiftr_no}
+    val ctxt = ctxt delsimps @{thms shiftr_no sshiftr_no shiftl_numeral}
         |> Splitter.del_split @{thm split_if}
         |> Simplifier.del_cong @{thm if_weak_cong}
 
@@ -435,14 +535,22 @@ fun graph_refine_proof_tacs csenv ctxt = let
                     var_ms_def init_vars_def
                     return_vars_def upd_vars_def save_vals_def
                     mem_upd_def mem_acc_def hrs_mem_update
+                    hrs_htd_update
+                    fupdate_def
 
-                    (* this includes wrappers for word arithmetic *)
+                    (* this includes wrappers for word arithmetic
+                       and other simpl actions*)
                     bvlshr_def bvashr_def bvshl_def bv_clz_def
+
+                    (* and some stupidity *)
+                    Collect_const_mem
                     }
                 (* we should also unfold enumerations, since the graph
                    representation does this, and we need to normalise
                    word arithmetic the same way on both sides. *)
                 addsimps (enum_simps csenv ctxt)
+                (* and fold up expanded array accesses *)
+                addsimprocs [fold_of_nat_eq_Ifs_simproc]
             )),
         (["step 3: split into goals with safe steps",
             "also derive ptr_safe assumptions from h_t_valid"],
@@ -453,38 +561,34 @@ fun graph_refine_proof_tacs csenv ctxt = let
         decompose_mem_goals false ctxt),
         (["step 5: normalise memory reads"],
         normalise_mem_accs ctxt),
+        (["step 6: explicitly apply some inequalities"],
+        TRY o DETERM o REPEAT_ALL_NEW
+            (eqsubst_either_wrap_tac ctxt @{thms word32_truncate_noop})),
         (["step 7: try to simplify out all remaining word logic"],
         asm_full_simp_tac (ctxt addsimps @{thms
                         pvalid_def pweak_valid_def palign_valid_def
                         field_lvalue_offset_eq array_ptr_index_def ptr_add_def
                         mask_def unat_less_helper
                         word_sle_def[THEN iffD2] word_sless_alt[THEN iffD2]
-                        field_simps NULL_ptr_val
                         drop_sign_isomorphism max_word_minus
                         ptr_equalities_to_ptr_val
                         extra_sle_sless_unfolds
                         word_neq_0_conv_neg_conv
+                        ucast_nat_def
+                        (* ucast_id *) scast_id of_int_sint_scast
+                        ptr_val_inj[symmetric]
+                        fold_all_htd_updates
                 }
+                delsimps @{thms ptr_val_inj}
             )),
-        (["step 8: attack unat less-than properties explicitly"],
+        (["step 8: try rewriting ring equalitites",
+            "this must be done after general simplification",
+            "because of a bug in the simpset for 2 ^ n",
+            "(unfolded in Suc notation if addition is commuted)"],
+        asm_full_simp_tac (ctxt addsimps @{thms field_simps})),
+        (["step 9: attack unat less-than properties explicitly"],
         TRY o unat_mono_tac ctxt)
 
-(* not sure if any of this is useful.
-        asm_full_simp_tac (ctxt addsimps @{thms
-                        to_bytes_array heap_update_def
-                        upt_rec take_heap_list_min drop_heap_list_general
-                        heap_update_list_append heap_list_update_ptr heap_list_update_word32
-                        store_store_word32_commute_offset field_simps
-                        heap_access_Array_element h_val_word32 h_val_ptr
-                        ucast_eq_0s}
-                    addsimps (Proof_Context.get_thms ctxt "field_h_val_rewrites")
-                    addsimps (Proof_Context.get_thms ctxt "field_to_bytes_rewrites")
-                ),
-        simp_tac (ctxt addsimps @{thms store_word32s_equality_fold
-                store_word32s_equality_final add_commute}),
-        simp_tac (ctxt addsimprocs [store_word32s_equality_simproc]
-            addsimps @{thms store_word32s_equality_final add_commute})
-*)
     ]
 
   end
